Updates.

HandbookOfPracticalLogicLean/Chapter2/NF/DNF/PureDNF.lean
@@ -28,9 +28,9 @@ def to_dnf_v3_aux_1 :
   Helper function for `to_dnf_v3`.
 -/
 def to_dnf_v3_aux_2
-  (ll : List (List Formula_)) :
+  (FSS : List (List Formula_)) :
   Formula_ :=
-  list_disj (List.map list_conj ll)
+  list_disj (List.map list_conj FSS)
 
 
 /--
@@ -171,14 +171,14 @@ lemma to_dnf_v3_aux_2_singleton
 
 lemma mem_list_mem_to_dnf_v3_aux_1_of_nnf_rec_v1_imp_is_constant_or_literal
   (F : Formula_)
-  (l : List Formula_)
-  (p : Formula_)
+  (PS : List Formula_)
+  (P : Formula_)
   (h1 : is_nnf_rec_v1 F)
-  (h2 : l ∈ to_dnf_v3_aux_1 F)
-  (h3 : p ∈ l) :
-  is_constant_ind p ∨ is_literal_ind p :=
+  (h2 : PS ∈ to_dnf_v3_aux_1 F)
+  (h3 : P ∈ PS) :
+  is_constant_ind P ∨ is_literal_ind P :=
   by
-  induction F generalizing l
+  induction F generalizing PS
   case false_ =>
     unfold to_dnf_v3_aux_1 at h2
     simp only [List.mem_singleton] at h2
@@ -230,22 +230,22 @@ lemma mem_list_mem_to_dnf_v3_aux_1_of_nnf_rec_v1_imp_is_constant_or_literal
 
     unfold to_dnf_v3_aux_1 at h2
 
-    obtain s1 := mem_all_pairs_v4_union_imp_eq_union (to_dnf_v3_aux_1 phi) (to_dnf_v3_aux_1 psi) l h2
-    obtain ⟨l1, l2, l1_mem, l2_mem, eq⟩ := s1
+    obtain s1 := mem_all_pairs_v4_union_imp_eq_union (to_dnf_v3_aux_1 phi) (to_dnf_v3_aux_1 psi) PS h2
+    obtain ⟨PS_1, PS_2, PS_1_mem, PS_2_mem, eq⟩ := s1
 
     rewrite [← eq] at h3
     simp only [List.mem_union_iff] at h3
 
     cases h3
     case inl h3 =>
-      apply phi_ih l1
+      apply phi_ih PS_1
       · exact h1_left
-      · exact l1_mem
+      · exact PS_1_mem
       · exact h3
     case inr h3 =>
-      apply psi_ih l2
+      apply psi_ih PS_2
       · exact h1_right
-      · exact l2_mem
+      · exact PS_2_mem
       · exact h3
   case or_ phi psi phi_ih psi_ih =>
     unfold is_nnf_rec_v1 at h1
@@ -256,12 +256,12 @@ lemma mem_list_mem_to_dnf_v3_aux_1_of_nnf_rec_v1_imp_is_constant_or_literal
 
     cases h2
     case inl h2 =>
-      apply phi_ih l
+      apply phi_ih PS
       · exact h1_left
       · exact h2
       · exact h3
     case inr h2 =>
-      apply psi_ih l
+      apply psi_ih PS
       · exact h1_right
       · exact h2
       · exact h3
